@prefix : <https://w3id.org/pko/audit/external#> .
@prefix owl: <http://www.w3.org/2002/07/owl#> .
@prefix pko: <https://w3id.org/pko#> .
@prefix rdf: <http://www.w3.org/1999/02/22-rdf-syntax-ns#> .
@prefix xml: <http://www.w3.org/XML/1998/namespace> .
@prefix xsd: <http://www.w3.org/2001/XMLSchema#> .
@prefix dcam: <http://purl.org/dc/dcam/> .
@prefix rdfs: <http://www.w3.org/2000/01/rdf-schema#> .
@prefix skos: <http://www.w3.org/2004/02/skos/core#> .
@prefix pko-aud: <https://w3id.org/pko/audit#> .
@base <https://w3id.org/pko/audit/external#> .

<https://w3id.org/pko/audit/external#> rdf:type owl:Ontology ;
                                        owl:imports <https://w3id.org/pko/audit> .

#################################################################
#    Annotation properties
#################################################################

###  http://purl.org/dc/dcam/domainIncludes
dcam:domainIncludes rdf:type owl:AnnotationProperty .


###  http://purl.org/dc/dcam/rangeIncludes
dcam:rangeIncludes rdf:type owl:AnnotationProperty .


###  http://www.w3.org/2004/02/skos/core#scopeNote
skos:scopeNote rdf:type owl:AnnotationProperty .


###  http://xmlns.com/foaf/0.1/name
<http://xmlns.com/foaf/0.1/name> rdf:type owl:AnnotationProperty .


#################################################################
#    Classes
#################################################################

###  http://xmlns.com/foaf/0.1/Organization
<http://xmlns.com/foaf/0.1/Organization> rdf:type owl:Class .


###  http://xmlns.com/foaf/0.1/Person
<http://xmlns.com/foaf/0.1/Person> rdf:type owl:Class .


#################################################################
#    Individuals
#################################################################

###  https://orcid.org/0000-0001-9962-7193
<https://orcid.org/0000-0001-9962-7193> rdf:type owl:NamedIndividual ,
                                                 <http://xmlns.com/foaf/0.1/Person> ;
                                        <http://xmlns.com/foaf/0.1/name> "Irene Celino"@en .


###  https://orcid.org/0000-0002-8235-7331
<https://orcid.org/0000-0002-8235-7331> rdf:type owl:NamedIndividual ,
                                                 <http://xmlns.com/foaf/0.1/Person> ;
                                        <http://xmlns.com/foaf/0.1/name> "Mario Scrocca"@en .


###  https://orcid.org/0000-0003-1427-3723
<https://orcid.org/0000-0003-1427-3723> rdf:type owl:NamedIndividual ,
                                                 <http://xmlns.com/foaf/0.1/Person> ;
                                        <http://xmlns.com/foaf/0.1/name> "Valentina Anita Carriero"@en .


###  https://ror.org/046bfkz44
<https://ror.org/046bfkz44> rdf:type owl:NamedIndividual ,
                                     <http://xmlns.com/foaf/0.1/Organization> ;
                            <http://xmlns.com/foaf/0.1/name> "Cefriel"@en .


#################################################################
#    Annotations
#################################################################

pko-aud:AuditBundle rdfs:comment "This class represents a Bundle that is generated during the Procedure Execution thanks to an Auditable System, and that may be collected by an Audit Service."@en ;
                    skos:scopeNote "In the context of the Procedural Knowledge Ontology, this class represents a Bundle that is generated during the Procedure Execution thanks to an Auditable System, and that may be collected by an Audit Service."@en .


pko-aud:AuditService rdfs:comment "This class represents a Service that performs auditing, and collects Audit Bundles that are sent by an Auditable System."@en ;
                     skos:scopeNote "In the context of the Procedural Knowledge Ontologu (PKO), this class represents a Service that performs auditing, and collects Audit Bundles that are sent by an Auditable System."@en .


pko-aud:AuditableProcedure rdfs:comment "This class represents a Procedure that can be audited, meaning that it can be executed involving a System that can send Bundles needed for performing auditing."@en ;
                           skos:scopeNote "In the context of the Procedural Knowledge Ontology, this class represents a Procedure that can be audited, meaning that it can be executed involving a System that can send Bundles needed for performing auditing."@en .


pko-aud:AuditableSystem rdfs:comment "Tthis class represents a System that can be involved in a Procedure Execution and can send Bundles needed for performing auditing."@en ;
                        skos:scopeNote "In the context of the Procedural Knowledge Ontology, this class represents a System that can be involved in a Procedure Execution and can send Bundles needed for performing auditing."@en .


pko-aud:hasAuditableProcedure rdfs:comment "In the context of the Procedural Knowledge Ontology (PKO), this property is used to link an Auditable System to an Auditable Procedure."@en ;
                              skos:scopeNote "In the context of the Procedural Knowledge Ontology (PKO), this property is used to link an Auditable System to an Auditable Procedure."@en .


pko-aud:hasAuditableSystem rdfs:comment "In the context of the Procedural Knowledge Ontology (PKO), this property is used to link an Auditable Procedur to an Auditable System."@en ;
                           skos:scopeNote "In the context of the Procedural Knowledge Ontology (PKO), this property is used to link an Auditable Procedur to an Auditable System."@en .


pko-aud:hasService rdfs:comment "In the context of the Procedural Knowledge Ontology (PKO), this property is used to link an Auditable System to an Audit Service."@en ;
                   skos:scopeNote "In the context of the Procedural Knowledge Ontology (PKO), this property is used to link an Auditable System to an Audit Service."@en .


pko-aud:isServiceFor rdfs:comment "In the context of the Procedural Knowledge Ontology (PKO), this property is used to link an Audit Service to an Auditable System."@en ;
                     skos:scopeNote "In the context of the Procedural Knowledge Ontology (PKO), this property is used to link an Audit Service to an Auditable System."@en .


pko-aud:wasCollectedBy skos:scopeNote "In the context of the Procedural Knowledge Ontology (PKO), this property is used to link an Audit Bundle to an Audit Service."@en .


###  Generated by the OWL API (version 4.5.26.2023-07-17T20:34:13Z) https://github.com/owlcs/owlapi
