@prefix : <https://w3id.org/pko/industry/external#> .
@prefix owl: <http://www.w3.org/2002/07/owl#> .
@prefix pko: <https://w3id.org/pko#> .
@prefix rdf: <http://www.w3.org/1999/02/22-rdf-syntax-ns#> .
@prefix xml: <http://www.w3.org/XML/1998/namespace> .
@prefix xsd: <http://www.w3.org/2001/XMLSchema#> .
@prefix dcam: <http://purl.org/dc/dcam/> .
@prefix rdfs: <http://www.w3.org/2000/01/rdf-schema#> .
@prefix skos: <http://www.w3.org/2004/02/skos/core#> .
@prefix pko-ind: <https://w3id.org/pko/industry#> .
@base <https://w3id.org/pko/industry/external#> .

<https://w3id.org/pko/industry/external#> rdf:type owl:Ontology ;
                                  owl:imports <https://w3id.org/pko/industry> .

#################################################################
#    Annotation properties
#################################################################

###  http://purl.org/dc/dcam/domainIncludes
dcam:domainIncludes rdf:type owl:AnnotationProperty .


###  http://purl.org/dc/dcam/rangeIncludes
dcam:rangeIncludes rdf:type owl:AnnotationProperty .


###  http://www.w3.org/2004/02/skos/core#scopeNote
skos:scopeNote rdf:type owl:AnnotationProperty .


pko-ind:Device rdfs:comment "This class represents a Device."@en .


pko-ind:EnergySource rdfs:comment "This class represents an Energy Source, that is a source of energy on the machine that needs to be identified and isolated during the LOTO procedure."@en .


pko-ind:Factory rdfs:comment "This class represents a building or set of buildings with facilities for manufacturing."@en .


pko-ind:Machine rdfs:comment "This class represents a Machine."@en .


pko-ind:MachineType rdfs:comment "This class represents the Type of a Machine."@en ;
                    skos:scopeNote "In the context of the Procedural Knowledge Ontology (PKO), this class represents the Machine Type of a Machine."@en .


pko-ind:Padlock rdfs:comment "This class represents a Padlock, that is a lock to be attached to the machine in order to prevent their re-activation, during the execution of a LOTO procedure."@en .


pko-ind:PersonalProtectiveEquipment rdfs:comment "This class represents a Personal Protective Equipment."@en .


pko-ind:hasMachineType rdfs:comment "This property is used to link a Machine to its Machine Type."@en ;
                        skos:scopeNote "In the context of the Procedural Knowledge Ontology (PKO), this property is used to link a Machine to the Machine Type."@en .


pko-ind:requiresPPE rdfs:comment "This property is used to link a Step to the Personal Protective Equipment (PPE) that is required by the Step."@en ;
                    skos:scopeNote "In the context of the Procedural Knowledge Ontology (PKO), this property is used to link a Step to the Personal Protective Equipment (PPE) that is required by the Step."@en .


pko-ind:requiresPadlock rdfs:comment "This property is used to link a Step to the Padlock it requires."@en ;
                        skos:scopeNote "In the context of the Procedural Knowledge Ontology (PKO), this property is used to link a Step to the Padlock it requires."@en .


pko-ind:wasManufacturedBy rdfs:comment "This property is used to link a Machine to the Agent that manufactured it."@en ;
                        skos:scopeNote "In the context of the Procedural Knowledge Ontology (PKO), this property is used to link a Machine to the Agent that manufactured it."@en .

pko-ind:isExecutedOnMachine rdfs:comment "This property is used to link an Activity (e.g., a Step Execution) to the Machine it is executed on."@en ;
                        skos:scopeNote "In the context of the Procedural Knowledge Ontology (PKO), this property is used to link an Activity (e.g., a Step Execution) to the Machine it is executed on."@en .

###  Generated by the OWL API (version 4.5.26.2023-07-17T20:34:13Z) https://github.com/owlcs/owlapi
