@prefix : <https://w3id.org/pko/external#> .
@prefix owl: <http://www.w3.org/2002/07/owl#> .
@prefix pko: <https://w3id.org/pko#> .
@prefix rdf: <http://www.w3.org/1999/02/22-rdf-syntax-ns#> .
@prefix xml: <http://www.w3.org/XML/1998/namespace> .
@prefix xsd: <http://www.w3.org/2001/XMLSchema#> .
@prefix dcam: <http://purl.org/dc/dcam/> .
@prefix rdfs: <http://www.w3.org/2000/01/rdf-schema#> .
@prefix skos: <http://www.w3.org/2004/02/skos/core#> .
@prefix pko-ind: <https://w3id.org/pko/industry#> .
@base <https://w3id.org/pko/external#> .

<https://w3id.org/pko/external#> rdf:type owl:Ontology ;
                                  owl:imports <https://w3id.org/pko> ,
                                              <https://w3id.org/pko/industry> .

#################################################################
#    Annotation properties
#################################################################

###  http://purl.org/dc/dcam/domainIncludes
dcam:domainIncludes rdf:type owl:AnnotationProperty .


###  http://purl.org/dc/dcam/rangeIncludes
dcam:rangeIncludes rdf:type owl:AnnotationProperty .


###  http://www.w3.org/2004/02/skos/core#scopeNote
skos:scopeNote rdf:type owl:AnnotationProperty .


#################################################################
#    Object Properties
#################################################################

###  http://purl.org/net/p-plan#isStepOfPlan
<http://purl.org/net/p-plan#isStepOfPlan> owl:inverseOf pko:hasStep ;
                                          dcam:domainIncludes <http://purl.org/net/p-plan#Step> ,
                                                              pko:Procedure ;
                                          skos:scopeNote "In the context of the Procedural Knowledge Ontology (PKO), this property is used to link a Step to the Procedure it is a step of."@en .


###  http://www.w3.org/ns/dcat#hasCurrentVersion
<http://www.w3.org/ns/dcat#hasCurrentVersion> owl:inverseOf pko:isCurrentVersionOf ;
                                              dcam:domainIncludes pko:Procedure ;
                                              dcam:rangeIncludes pko:Procedure ;
                                              skos:scopeNote "In the context of the Procedural Knowledge Ontology (PKO), this property is used to link a Procedure, for which we want to manage version control, to its current version."@en .


###  http://www.w3.org/ns/dcat#previousVersion
<http://www.w3.org/ns/dcat#previousVersion> owl:inverseOf pko:nextVersion ;
                                            dcam:domainIncludes pko:Procedure ;
                                            dcam:rangeIncludes pko:Procedure ;
                                            skos:scopeNote "In the context of the Procedural Knowledge Ontology (PKO), this property is used to link a version of a Procedure to its direct previous version of the same Procedure."@en .


###  http://www.w3.org/ns/prov#wasAssociatedWith
<http://www.w3.org/ns/prov#wasAssociatedWith> dcam:domainIncludes <http://www.w3.org/ns/prov#Activity> ;
                                              dcam:rangeIncludes <http://www.w3.org/ns/prov#Agent> ;
                                              skos:scopeNote "In the context of the Procedural Knowledge Ontology (PKO), this property is used to link an Activity (either a Procedure Execution or a Step Execution) to an Agent that had some role/responsibility in that Activity."@en .


###  https://w3id.org/pko#hasStep
pko:hasStep skos:scopeNote "In the context of the Procedural Knowledge Ontology (PKO), this property is used to link a Procedure or a MultiStep to its Steps."@en .


###  https://w3id.org/pko#hasStepVerification
pko:hasStepVerification owl:inverseOf pko:isStepVerificationOf ;
                        skos:scopeNote "In the context of the Procedural Knowledge Ontology (PKO), this property is used to link a Step of a Procedure to a Step Verification, that is the way in which the execution of the step can be verified."@en .


###  https://w3id.org/pko#isStepVerificationOf
pko:isStepVerificationOf skos:scopeNote "In the context of the Procedural Knowledge Ontology (PKO), this property is used to link a Step Verification, that is the way in which the execution of the step can be verified, to the Step it verifies."@en .


###  https://w3id.org/pko#nextStep
pko:nextStep owl:inverseOf pko:previousStep ;
             skos:scopeNote "In the context of the Procedural Knowledge Ontology (PKO), this property is used to link a Step to its direct next Step."@en .


###  https://w3id.org/pko#nextStepExecution
pko:nextStepExecution owl:inverseOf pko:previousStepExecution ;
                      skos:scopeNote "In the context of the Procedural Knowledge Ontology (PKO), this property is used to link a Step Execution to its direct next Step Execution."@en .


###  https://w3id.org/pko#nextVersion
pko:nextVersion skos:scopeNote "In the context of the Procedural Knowledge Ontology (PKO), this property is used to link a version of a Procedure to its direct next version of the same Procedure."@en .


###  https://w3id.org/pko#previousStep
pko:previousStep skos:scopeNote "In the context of the Procedural Knowledge Ontology (PKO), this property is used to link a Step to its direct previous Step."@en .


###  https://w3id.org/pko#previousStepExecution
pko:previousStepExecution skos:scopeNote "In the context of the Procedural Knowledge Ontology (PKO), this property is used to link a Step Execution to its direct previous Step Execution."@en .


###  https://w3id.org/pko#wasConfirmedBy
pko:wasConfirmedBy rdfs:subPropertyOf <http://www.w3.org/ns/prov#wasAssociatedWith> .


###  https://w3id.org/pko#wasExecutedBy
pko:wasExecutedBy rdfs:subPropertyOf <http://www.w3.org/ns/prov#wasAssociatedWith> .


#################################################################
#    Annotations
#################################################################

<http://purl.org/dc/terms/created> dcam:domainIncludes <http://www.w3.org/ns/dcat#Resource> ;
                                   dcam:rangeIncludes xsd:dateTime ;
                                   skos:scopeNote "In the context of the Procedural Knowledge Ontology (PKO), this property is used to represent the creation dateTime of a Resource (e.g., a Procedure)."@en .


<http://purl.org/dc/terms/creator> dcam:domainIncludes <http://www.w3.org/ns/dcat#Resource> ;
                                   dcam:rangeIncludes <http://www.w3.org/ns/prov#Agent> ;
                                   skos:scopeNote "In the context of the Procedural Knowledge Ontology (PKO), this property is used to link a Resource (e.g., a Procedure) to the Agent that created it."@en .


<http://purl.org/dc/terms/description> dcam:domainIncludes <http://www.w3.org/ns/dcat#Resource> ,
                                                           <http://www.w3.org/ns/prov#Activity> ;
                                       dcam:rangeIncludes xsd:string ;
                                       skos:scopeNote "In the context of the Procedural Knowledge Ontology (PKO), this property is used to represent a description of an entity, including: a Procedure, a Step, a Procedure Execution, a Step Execution, a Step Verification, a Resource that is referenced by or which a Procedure was extracted from."@en .


<http://purl.org/dc/terms/format> dcam:domainIncludes <http://purl.org/dc/terms/MediaTypeOrExtent> ,
                                                      <http://www.w3.org/ns/dcat#Resource> ;
                                  skos:scopeNote "In the context of the Procedural Knowledge Ontology (PKO), this property is used to link a Resource (e.g., a Procedure or a Resource referenced by a Procedure), to the Media Type or Extent of the resource."@en .


<http://purl.org/dc/terms/identifier> dcam:domainIncludes <http://www.w3.org/ns/dcat#Resource> ;
                                      dcam:rangeIncludes xsd:string ;
                                      skos:scopeNote "In the context of the Procedural Knowledge Ontology (PKO), this property is used to represent the identifier of an entity, including: a Procedure, a Step, a Procedure Execution, a Step Execution, a Step Verification, a FAQ Category, a FAQ Target, a Resource that is referenced by or which a Procedure was extracted from."@en .


<http://purl.org/dc/terms/language> dcam:domainIncludes <http://www.w3.org/ns/dcat#Resource> ;
                                    dcam:rangeIncludes xsd:string ;
                                    skos:scopeNote "In the context of the Procedural Knowledge Ontology (PKO), this property is used to represent the language of a Resource (e.g., a Procedure)."@en .


<http://purl.org/dc/terms/modified> dcam:domainIncludes <http://www.w3.org/ns/dcat#Resource> ;
                                    dcam:rangeIncludes xsd:dateTime ;
                                    skos:scopeNote "In the context of the Procedural Knowledge Ontology (PKO), this property is used to represent the dateTime when a Resource  (e.g., a Procedure) has been modified."@en .


<http://purl.org/dc/terms/references> dcam:domainIncludes <http://www.w3.org/ns/dcat#Resource> ;
                                      dcam:rangeIncludes <http://www.w3.org/ns/dcat#Resource> ;
                                      skos:scopeNote "In the context of the Procedural Knowledge Ontology (PKO), this property is used to link a Resource (e.g., a Procedure) to another Resource (e.g., a document, an image, or another Procedure) that the Procedure references."@en .


<http://purl.org/dc/terms/temporal> dcam:domainIncludes <http://purl.org/spar/pro/RoleInTime> ;
                                    dcam:rangeIncludes <http://purl.org/dc/terms/PeriodOfTime> ;
                                    skos:scopeNote "In the context of the Procedural Knowledge Ontology (PKO), this property is used to link a Role In Time held by an Agent to the Period of Time in which that Role is valid."@en .


<http://purl.org/dc/terms/title> dcam:domainIncludes <http://www.w3.org/ns/dcat#Resource> ;
                                 dcam:rangeIncludes xsd:string ;
                                 skos:scopeNote "In the context of the Procedural Knowledge Ontology (PKO), this property is used to represent the name/title of an entity, including: a Procedure, a Step, a Procedure Execution, a Step Execution, a Step Verification, a FAQ Category, a FAQ Target, a Resource that is referenced by or which a Procedure was extracted from."@en .


<http://purl.org/net/p-plan#correspondsToVariable> dcam:domainIncludes <http://www.w3.org/ns/prov#Entity> ;
                                                   dcam:rangeIncludes <http://purl.org/net/p-plan#Variable> ;
                                                   skos:scopeNote "In the context of the Procedural Knowledge Ontology (PKO), this property is used to link an Entity used by an Activity (either a Procedure Execution or a Step Execution) to the Variable it represented in the Procedure."@en .


<http://purl.org/net/p-plan#hasInputVar> dcam:domainIncludes <http://purl.org/net/p-plan#Step> ;
                                         dcam:rangeIncludes <http://purl.org/net/p-plan#Variable> ;
                                         skos:scopeNote "In the context of the Procedural Knowledge Ontology (PKO), this property is used to link a Step to the Variable that the Step needs to take as input for the Step Execution."@en .


<http://purl.org/net/p-plan#hasOutputVar> dcam:domainIncludes <http://purl.org/net/p-plan#Step> ;
                                          dcam:rangeIncludes <http://purl.org/net/p-plan#Variable> ;
                                          skos:scopeNote "In the context of the Procedural Knowledge Ontology (PKO), this property is used to link a Step to the Variable that the Step needs to produce as output of the Step Execution."@en .


<http://purl.org/spar/pro/holdsRoleInTime> dcam:domainIncludes <http://www.w3.org/ns/prov#Agent> ;
                                           dcam:rangeIncludes <http://purl.org/spar/pro/RoleInTime> ;
                                           skos:scopeNote "In the context of the Procedural Knowledge Ontology (PKO), this property is used to link an Agent to the Role In Time, that is the role that the Agent holds for a certain Period of Time."@en .


<http://purl.org/spar/pro/relatesTo> dcam:domainIncludes <http://purl.org/spar/pro/RoleInTime> ;
                                     dcam:rangeIncludes <http://www.w3.org/ns/dcat#Resource> ;
                                     skos:scopeNote "In the context of the Procedural Knowledge Ontology (PKO), this property is used to link a Role In Time, that is the role that an Agent holds for a certain Period of Time, to the Resource (e.g., a Procedure) that the Role relates to."@en .


<http://purl.org/spar/pro/withRole> dcam:domainIncludes <http://purl.org/spar/pro/RoleInTime> ;
                                    dcam:rangeIncludes <http://purl.org/spar/pro/Role> ;
                                    skos:scopeNote "In the context of the Procedural Knowledge Ontology (PKO), this property is used to link a Role In Time, that is the role that an Agent holds for a certain Period of Time, to the Role that is held."@en .


<http://w3id.org/nfdi4ing/metadata4ing#Tool> skos:scopeNote "In the context of the Procedural Knowledge Ontology (PKO), this class represents an object needed to execute a Step of a Procedure."@en .


<http://www.w3.org/2006/time#numericDuration> dcam:domainIncludes <http://www.w3.org/2006/time#Duration> ;
                                              dcam:rangeIncludes xsd:date ;
                                              skos:scopeNote "In the context of the Procedural Knowledge Ontology (PKO), this property is used to represent the value of a temporal extent expressed as a number scaled by a temporal unit (in the form of xsd:decimal)."@en .


<http://www.w3.org/2006/time#unitType> dcam:domainIncludes <http://www.w3.org/2006/time#Duration> ;
                                       dcam:rangeIncludes <http://www.w3.org/2006/time#TemporalUnit> ;
                                       skos:scopeNote "In the context of the Procedural Knowledge Ontology (PKO), this property is used to link a Duration of time to the Temporal Unit which provides the precision of a date-time value or scale of a temporal extent."@en .


<http://www.w3.org/ns/adms#status> dcam:domainIncludes <http://www.w3.org/ns/dcat#Resource> ;
                                   dcam:rangeIncludes pko:ProcedureStatus ;
                                   skos:scopeNote "In the context of the Procedural Knowledge Ontology (PKO), this property is used to link either a Procedure or a Procedure Execution to its Status."@en .


<http://www.w3.org/ns/dcat#accessURL> dcam:domainIncludes <http://www.w3.org/ns/dcat#Resource> ;
                                      skos:scopeNote "In the context of the Procedural Knowledge Ontology (PKO), this property is used to represent a URL of a Resource (e.g., a Procedure or a document referenced by a Procedure) that gives access to a distribution of it."@en .


<http://www.w3.org/ns/dcat#endDate> dcam:domainIncludes <http://purl.org/dc/terms/PeriodOfTime> ;
                                    dcam:rangeIncludes xsd:date ;
                                    skos:scopeNote "In the context of the Procedural Knowledge Ontology (PKO), this property is used to represent the end of a Period Of Time."@en .


<http://www.w3.org/ns/dcat#hasVersion> dcam:domainIncludes pko:Procedure ;
                                       dcam:rangeIncludes pko:Procedure ;
                                       skos:scopeNote "In the context of the Procedural Knowledge Ontology (PKO), this property is used to link a Procedure, for which we want to manage version control, to one of its versions."@en .


<http://www.w3.org/ns/dcat#isVersionOf> dcam:domainIncludes pko:Procedure ;
                                        dcam:rangeIncludes pko:Procedure ;
                                        skos:scopeNote "In the context of the Procedural Knowledge Ontology (PKO), this property is used to a version of a procedure to the Procedure, for which we want to manage version control."@en .


<http://www.w3.org/ns/dcat#keyword> dcam:domainIncludes <http://www.w3.org/ns/dcat#Resource> ;
                                    dcam:rangeIncludes xsd:string ;
                                    skos:scopeNote "In the context of the Procedural Knowledge Ontology (PKO), this property is used to represent a keyword or tag describing a Resource (e.g, a Procedure)."@en .


<http://www.w3.org/ns/dcat#startDate> dcam:domainIncludes <http://purl.org/dc/terms/PeriodOfTime> ;
                                      dcam:rangeIncludes xsd:date ;
                                      skos:scopeNote "In the context of the Procedural Knowledge Ontology (PKO), this property is used to represent the start of a Period Of Time."@en .


<http://www.w3.org/ns/prov#atLocation> skos:scopeNote "In the context of the Procedural Knowledge Ontology (PKO), this property is used to link a Procedure Target to the Location where is Target is located."@en .


<http://www.w3.org/ns/prov#atTime> dcam:domainIncludes <http://www.w3.org/ns/prov#InstantaneousEvent> ;
                                   dcam:rangeIncludes xsd:dateTime ;
                                   skos:scopeNote "In the context of the Procedural Knowledge Ontology (PKO), this property is used to represent the dateTime at which an InstantaneousEvent occurred."@en .


<http://www.w3.org/ns/prov#endedAtTime> dcam:domainIncludes <http://www.w3.org/ns/prov#Activity> ;
                                        dcam:rangeIncludes xsd:dateTime ;
                                        skos:scopeNote "In the context of the Procedural Knowledge Ontology (PKO), this property is used to represent the dateTime at which an activity ended."@en .


<http://www.w3.org/ns/prov#startedAtTime> dcam:domainIncludes <http://www.w3.org/ns/prov#Activity> ;
                                          dcam:rangeIncludes xsd:dateTime ;
                                          skos:scopeNote "In the context of the Procedural Knowledge Ontology (PKO), this property is used to represent the dateTime at which an activity started."@en .


<http://www.w3.org/ns/prov#used> dcam:domainIncludes pko:StepExecution ;
                                 dcam:rangeIncludes <http://www.w3.org/ns/prov#Entity> ;
                                 skos:scopeNote "In the context of the Procedural Knowledge Ontology (PKO), this property is used to link a Step Execution to an Entity that is being used during execution, and that may correspond to an input Variable of the Step."@en .


<http://www.w3.org/ns/prov#wasGeneratedBy> dcam:domainIncludes <http://www.w3.org/ns/prov#Entity> ;
                                           dcam:rangeIncludes pko:StepExecution ;
                                           skos:scopeNote "In the context of the Procedural Knowledge Ontology (PKO), this property is used to link a Step Execution to an Entity that was generated during execution, and that may correspond to an output Variable of the Step."@en .


pko:Action rdfs:comment "This class represents an Action performed by a human Agent."@en ;
           skos:scopeNote "In the context of the Procedural Knowledge Ontology (PKO), this class represents an action that needs to be performed by a human Agent (a Person) for executing a Step of a Procedure."@en .


pko:Error rdfs:comment "This class represents an Error that can be encountered while executing an activity."@en ;
          skos:scopeNote "In the context of the Procedural Knowledge Ontology (PKO), this class represents an error that an Agent can encounter during a Procedure or Step Execution. An Error can be associated with a description, an error code, and an error cause. The Procedure may contain a (fallback) step to address such error."@en .


pko:ExpertiseLevel rdfs:comment "This class represents the Expertise Level of an Agent with respect to certain activities/responsibilities."@en ;
                   skos:scopeNote "In the context of the Procedural Knowledge Ontology (PKO), this class represents the expertise level linked to a Step, or MultiStep, of a Procedure, meaning that the Step, or MultiStep, is targeted at persons with a certain level of expertise (e.g., junior, senior)."@en .


pko:FAQCategory rdfs:comment "This class represents the Category of a Frequently Asked Question (FAQ)."@en .


pko:FAQTarget rdfs:comment "This class represents the Target of a Frequently Asked Question (FAQ)."@en .


pko:FrequentlyAskedQuestion rdfs:comment "A Frequently Asked Question (FAQ) is a Resource representing a question that people often ask about a particular resource, and the answer to the question."@en ;
                            skos:scopeNote "In the context of the Procedural Knowledge Ontology (PKO), this class represents a Frequently Asked Question (FAQ) of a Procedure, and is described with an identifier, a question, an answer, and is linked to a FAQ Category and a FAQ Target."@en .


pko:Function rdfs:comment "This class represents a Function performed by a Software Agent."@en ;
             skos:scopeNote "In the context of the Procedural Knowledge Ontology (PKO), this class represents a function that needs to be performed by a Software Agent for executing a Step of a Procedure."@en .


pko:IssueOccurrence rdfs:comment "This class represents the occurrence of an issue during an Activity."@en ;
                    skos:scopeNote "In the context of the Procedural Knowledge Ontology (PKO), this class represents the occurrence of an issue during the Procedure or Step Execution. The Issue Occurrence is associated with the cause as identified and defined by the Agent, the solution as identified and applied by the Agent, and is linked to the Agent that encountered the issue."@en .


pko:Procedure rdfs:comment "A Procedure represents a sequence of actions to be executed in order to achieve a desired outcome."@en .


pko:ProcedureExecution rdfs:comment "A Procedure Execution is an Activity representing the execution of a certain Procedure, performed by one or more Agents, during a time interval."@en .


pko:ProcedureExecutionStatus rdfs:comment "This class represents the Status of the Procedure Execution (e.g., in progress, completed, paused, cancelled)."@en ;
                             skos:scopeNote "In the context of the Procedural Knowledge Ontology (PKO), a Procedure Execution is linked to its Procedure Execution Status with the property adms:status."@en .


pko:ProcedureStatus rdfs:comment "This class represents the Status of the Procedure (e.g.,draft, validated)."@en ;
                    skos:scopeNote "In the context of the Procedural Knowledge Ontology (PKO), a Procedure  is linked to its Procedure Status with the property adms:status."@en .


pko:ProcedureTarget rdfs:comment "This class represents the Target of a Procedure, that is the object at which the actions of the Procedure are directed."@en ;
                    skos:scopeNote "In the context of the Procedural Knowledge Ontology (PKO),  a Procedure Target can be, for instance: a Machine, an Equipment, a Workstation."@en .


pko:ProcedureTargetType rdfs:comment "This class represents the Type of a Procedure Target."@en .


pko:ProcedureType rdfs:comment "This class represents the Type of a Procedure."@en ;
                  skos:scopeNote "In the context of the Procedural Knowledge Ontology (PKO), an example of Procedure Type is LOTO Procedure."@en .


pko:StepExecution rdfs:comment "A Procedure Execution is an Activity representing the execution of a certain Step of a Procedure, performed by one or more Agents, during a time interval."@en .


pko:StepVerification rdfs:comment "A Step Verification is a description of the way in which the execution of a Step can be verified."@en .


pko:UserFeedbackOccurrence rdfs:comment "This class represents the occurrence of a feedback that was provided by a user during an activity."@en ;
                           skos:scopeNote "In the context of the Procedural Knowledge Ontology (PKO), this class represents the occurrence of a feedback provided by an Agent during the Procedure or Step Execution. The User Feedback Occurrence is associated with the feedback, that is about either the Procedure or the Procedure Execution, and is linked to the Agent providing the feedback."@en .


pko:UserQuestionOccurrence skos:scopeNote "In the context of the Procedural Knowledge Ontology (PKO), this class represents the occurrence of a question that an Agent came up with during the Procedure or Step Execution. The User Question Occurrence is associated with the question, and is linked to the Agent asking the question. Also, it can be linked to a Resource addressing the question."@en .


pko:addressesError skos:scopeNote "In the context of the Procedural Knowledge Ontology (PKO), this property is used to link a (Multi)Step of a Procedure to the Error it addresses. Such (Multi)Step represents a Fallback procedure."@en .


pko:answer skos:scopeNote "In the context of the Procedural Knowledge Ontology (PKO), this property is used to represent the answer of a Frequently Asked Question."@en .


pko:changelogDescription skos:scopeNote "In the context of the Procedural Knowledge Ontology (PKO), this property is used to represent the changelog description of a Procedure, that details all updates with respect to the previous version of the same Procedure."@en .


pko:errorCause skos:scopeNote "In the context of the Procedural Knowledge Ontology (PKO), this property is used to represent the cause of an Error that can be encountered during the Procedure or Step Execution."@en .


pko:errorCode skos:scopeNote "In the context of the Procedural Knowledge Ontology (PKO), this property is used to represent the code of an Error that can be encountered during the Procedure or Step Execution."@en .


pko:executesProcedure skos:scopeNote "In the context of the Procedural Knowledge Ontology (PKO), this property is used to link a Procedure Execution to the Procedure that is being executed."@en .


pko:executesStep skos:scopeNote "In the context of the Procedural Knowledge Ontology (PKO), this property is used to link a Step Execution to the Step that is being executed."@en .


pko:feedbackOnProcedure skos:scopeNote "In the context of the Procedural Knowledge Ontology (PKO), this property is used to represent the feedback on the procedure that was provided by an Agent during the Procedure or Step Execution."@en .


pko:feedbackOnProcedureExecution skos:scopeNote "In the context of the Procedural Knowledge Ontology (PKO), this property is used to represent the feedback on the procedure execution that was provided by an Agent during the Procedure or Step Execution."@en .


pko:hasEncounteredError skos:scopeNote "In the context of the Procedural Knowledge Ontology (PKO), this property is used to link the Occurrence of an Issue to the Error that is being encountered by the Agent executing a Procedure or Step."@en .


pko:hasExpectedDuration skos:scopeNote "In the context of the Procedural Knowledge Ontology (PKO), this property is used to link either a Procedure or a Step to the Duration that is expected for the execution of that Procedure/Step."@en .


pko:hasFAQCategory skos:scopeNote "In the context of the Procedural Knowledge Ontology (PKO), this property is used to link a Frequently Asked Question to a Category it belongs to."@en .


pko:hasFAQTarget skos:scopeNote "In the context of the Procedural Knowledge Ontology (PKO), this property is used to link a Frequently Asked Question to the Target of such FAQ."@en .


pko:hasFallbackStep skos:scopeNote "In the context of the Procedural Knowledge Ontology (PKO), this property is used to link a Procedure to a (Multi)Step that represents a Fallback procedure for a specific Error that can be encountered during execution."@en .


pko:hasFirstStep skos:scopeNote "In the context of the Procedural Knowledge Ontology (PKO), this property is used to link a Procedure or a MultiStep to its first Step."@en .


pko:hasIssueOccurrence skos:scopeNote "In the context of the Procedural Knowledge Ontology (PKO), this property is used to link a Procedure Execution or Step Execution to an Issue Occurrence, that is the occurrence of an issue during the execution."@en .


pko:hasProcedureTarget skos:scopeNote "In the context of the Procedural Knowledge Ontology (PKO), this property is used to link a Procedure to its Procedure Target(s), that is the object at which the actions of the Procedure are directed. A Procedure Target can be, for instance: a Machine, an Equipment, a Workstation."@en .


pko:hasProcedureTargetType skos:scopeNote "In the context of the Procedural Knowledge Ontology (PKO), this property is used to link a ProcedureTarget to its Procedure Target Type."@en .


pko:hasProcedureType skos:scopeNote "In the context of the Procedural Knowledge Ontology (PKO), this property is used to link a Procedure to its Procedure Type (e.g., a LOTO Procedure)."@en .


pko:hasUserFeedbackOccurrence skos:scopeNote "In the context of the Procedural Knowledge Ontology (PKO), this property is used to link a Procedure Execution to a User Feedback Occurrence, that is the occurrence of a feedback that the user provides during execution about wither the Procedure or the Procedure Execution."@en .


pko:hasUserQuestionOccurrence skos:scopeNote "In the context of the Procedural Knowledge Ontology (PKO), this property is used to link a Procedure Execution or Step Execution to a User Question Occurrence, that is the occurrence of a question that the user came up with during execution."@en .


pko:isAdoptedBy skos:scopeNote "In the context of the Procedural Knowledge Ontology (PKO), this property is used to link a Procedure to an Organization which the Procedure is adopted by."@en .


pko:isQuestionAddressedBy skos:scopeNote "In the context of the Procedural Knowledge Ontology (PKO), this property is used to link a User Question Occurrence to a Resource that addresses/answers to the question that the user came up with during the Procedure/Step Execution."@en .


pko:isStepForExpertiseLevel skos:scopeNote "In the context of the Procedural Knowledge Ontology (PKO), this property is used to link a Step to the Expertise Level, meaning that the Step, or MultiStep, is targeted at persons with a certain level of expertise (e.g., junior, senior)."@en .


pko:isStepOfMultiStep skos:scopeNote "In the context of the Procedural Knowledge Ontology (PKO), this property is used to link a Step to the MultiStep it is a step of."@en .


pko:isTemplate skos:scopeNote "In the context of the Procedural Knowledge Ontology (PKO), this property is used to represent whether a Procedure is a Template or not. A Procedure is a Template if it is associated with a preset of Steps that can be used to define an Executable Procedure. Such steps are not directly executable in the form they are specified."@en .


pko:issueCauseByUser skos:scopeNote "In the context of the Procedural Knowledge Ontology (PKO), this property is used to represent the cause of an issue, encountered during a Procedure/Step Execution, as identified and defined by the user."@en .


pko:issueSolutionByUser skos:scopeNote "In the context of the Procedural Knowledge Ontology (PKO), this property is used to represent the solution of an issue, encountered during a Procedure/Step Execution, as identified and applied by the user."@en .


pko:maxRepetitions skos:scopeNote "In the context of the Procedural Knowledge Ontology (PKO), this property is used to represent the maximum number of repetitions for a Step. If the maxRepetitions is equal to 1, it means that the Step is not repeatable."@en .


pko:minRepetitions skos:scopeNote "In the context of the Procedural Knowledge Ontology (PKO), this property is used to represent the maximum number of repetitions for a Step. If the minRepetitions is equal to 1, it means that the Step is mandatory. If the minRepetitions is equal to 0, it means that the Step is optional."@en .


pko:newVersionMotivation skos:scopeNote "In the context of the Procedural Knowledge Ontology (PKO), this property is used to represent the motivation for creating a new version of a Procedure, for which we want to manage access control."@en .


pko:nextAlternativeStep skos:scopeNote "In the context of the Procedural Knowledge Ontology (PKO), this property is used to link a Step to at least two alternative Steps, if only one of such steps should be executed."@en .


pko:notesByUser skos:scopeNote "In the context of the Procedural Knowledge Ontology (PKO), this property is used to represent the notes taken by the user about either a question that occurred during the Procedure/Step Execution (User Question Occurrence) or an issue that occurred during the Procedure/Step Execution (Issue Occurrence)."@en .


pko:question skos:scopeNote "In the context of the Procedural Knowledge Ontology (PKO), this property is used to represent the question of a Frequently Asked Question."@en .


pko:questionByUser skos:scopeNote "In the context of the Procedural Knowledge Ontology (PKO), this property is used to represent the question that a user came up with during the Procedure/Step Execution (User Question Occurrence)."@en .


pko:requiresAction skos:scopeNote "In the context of the Procedural Knowledge Ontology (PKO), this property is used to link a Step to an Action that needs to be performed by a human Agent (a Person) for executing the Step."@en .


pko:requiresFunction skos:scopeNote "In the context of the Procedural Knowledge Ontology (PKO), this property is used to link a Step to a Function that needs to be performed by a Software Agent for executing the Step."@en .


pko:requiresTool skos:scopeNote "In the context of the Procedural Knowledge Ontology (PKO), this property is used to link a Step of a Procedure to a Tool required by the Step, that is an object needed to execute the Step."@en .


pko:versionNumber skos:scopeNote "In the context of the Procedural Knowledge Ontology (PKO), this property is used to represent the number of the version of a Procedure, for which we want to manage access control."@en .


pko:wasAskedBy skos:scopeNote "In the context of the Procedural Knowledge Ontology (PKO), this property is used to link a User Question Occurrence to the Agent that asked the question during the Procedure/Step Execution."@en .


pko:wasEncounteredBy skos:scopeNote "In the context of the Procedural Knowledge Ontology (PKO), this property is used to link an Issue Occurrence to the Agent that encountered the issue during the Procedure/Step Execution."@en .


pko:wasExtractedFrom skos:scopeNote "In the context of the Procedural Knowledge Ontology (PKO), this property is used to link a Resource (e.g., a Procedure) to the Resource it was extracted from."@en .


pko:wasModifiedBy skos:scopeNote "In the context of the Procedural Knowledge Ontology (PKO), this property is used to link a Resource (e.g., a Procedure) to the Agent that modified the Resource."@en .


pko:wasProvidedBy skos:scopeNote "In the context of the Procedural Knowledge Ontology (PKO), this property is used to link a User Feedback Occurrence to the Agent that provided the feedback about either the procedure or the procedure execution during the Procedure Execution."@en .


pko-ind:Device rdfs:comment "This class represents a Device."@en .


pko-ind:EnergySource rdfs:comment "This class represents an Energy Source, that is a source of energy on the machine that needs to be identified and isolated during the LOTO procedure."@en .


pko-ind:Factory rdfs:comment "This class represents a building or set of buildings with facilities for manufacturing."@en .


pko-ind:Machine rdfs:comment "This class represents a Machine."@en .


pko-ind:MachineType rdfs:comment "This class represents the Type of a Machine."@en ;
                    skos:scopeNote "In the context of the Procedural Knowledge Ontology (PKO), this class represents the Machine Type of a Machine."@en .


pko-ind:Padlock rdfs:comment "This class represents a Padlock, that is a lock to be attached to the machine in order to prevent their re-activation, during the execution of a LOTO procedure."@en .


pko-ind:PersonalProtectiveEquipment rdfs:comment "This class represents a Personal Protective Equipment."@en .


pko-ind:hasMachineType skos:scopeNote "In the context of the Procedural Knowledge Ontology (PKO), this property is used to link a Machine to the Machine Type."@en .


pko-ind:requiresPPE skos:scopeNote "In the context of the Procedural Knowledge Ontology (PKO), this property is used to link a Step to the Personal Protective Equipment (PPE) that is required by the Step."@en .


pko-ind:requiresPadlock skos:scopeNote "In the context of the Procedural Knowledge Ontology (PKO), this property is used to link a Step to the Padlock it requires."@en .


pko-ind:wasManufacturedBy skos:scopeNote "In the context of the Procedural Knowledge Ontology (PKO), this property is used to link a Machine to the Agent that manufactured it."@en .


###  Generated by the OWL API (version 4.5.26.2023-07-17T20:34:13Z) https://github.com/owlcs/owlapi
